Automata/Test.lean
@@ -1,9 +1,0 @@
-import Mathlib.Data.Real.Basic
-import Mathlib.Tactic
-
-set_option trace.profiler true
-
-theorem foo : 2 + 3 = 5 := by rfl
-
-
-#eval 2 + 2
